Define and benchmark [equations_blit].

src/array.v
@@ -1008,6 +1008,42 @@ Proof.
     isArray. }
 Qed.
 
+(* In order to allow a fair comparison, let's define a third naive [blit],
+   this time using Equations, but without a higher-order function. *)
+
+Section Code.
+Open Scope uint63.
+
+Equations equations_blit a _i b _j _n : array A
+by wf _n ilt :=
+equations_blit a _i b _j _n :=
+  IF _n =? 0 THEN
+    b
+  ELSE
+    do x ← get a _i ;
+    do b ← set b _j x ;
+    equations_blit a (_i + 1) b (_j + 1) (_n - 1).
+
+End Code.
+
+(* We can now prove that [equations_blit] is correct. *)
+
+Lemma wp_equations_blit _n :
+  blit_spec (λ a _i b _j, equations_blit a _i b _j _n) _n.
+Proof.
+  (* By well-founded induction on [_n]. *)
+  pattern _n. eapply (well_founded_ind ilt_wf). clear _n. intros _n IH.
+  unfold blit_spec. intros. autorewrite with equations_blit.
+  wp_if.
+  (* Base case. *)
+  { wp_ret. isArray. }
+  (* Step case. *)
+  { wp_get x.
+    wp_set.
+    wp_op IH; last wp_shadow b.
+    isArray. }
+Qed.
+
 (* TODO *)
 Definition blit := @simple_blit.
 Definition wp_blit := @wp_simple_blit.
